Make MinimalParse compile

src/Parsers/MinimalParse.v
@@ -571,14 +571,12 @@ Section cfg.
               + alt_option (size_of_parse_item (ParseNonTerminal name p)) valid str.
 
       Section item.
-        Context {str0 str : String} {valid : names_listT}
-                (Hinit : sub_names_listT valid initial_names_data).
+        Context {str0 str : String} {valid : names_listT}.
 
         Definition minimal_parse_of_item__of__parse_of_item
                    h
                    (minimal_parse_of_name__of__parse_of_name
                     : forall h' (pf : h' < S (S h)) {str0 str valid name}
-                             (Hinit : sub_names_listT valid initial_names_data)
                              (p : parse_of String G str (Lookup G name)),
                         @of_parse_name_T str0 str valid name p h')
         : of_parse_item_T str h.
@@ -589,7 +587,7 @@ Section cfg.
           { left.
             eexists (MinParseTerminal _ _ _);
               split; simpl; constructor. }
-          { edestruct (fun pf pf' => @minimal_parse_of_name__of__parse_of_name (S h') pf str _ valid' _ pf' p') as [ [p'' H''] | p'' ];
+          { edestruct (fun pf => @minimal_parse_of_name__of__parse_of_name (S h') pf str _ valid' _ p') as [ [p'' H''] | p'' ];
             try solve [ repeat (apply Lt.lt_n_Sn || apply Lt.lt_S)
                       | exact Hinit'
                       | exact H_h
@@ -605,8 +603,7 @@ Section cfg.
       End item.
 
       Section production.
-        Context {str0 str : String} {valid : names_listT}
-                (Hinit : sub_names_listT valid initial_names_data).
+        Context {str0 str : String} {valid : names_listT}.
 
         Local Ltac min_parse_prod_t' :=
           idtac;
@@ -694,7 +691,6 @@ Section cfg.
                  h
                  (minimal_parse_of_name__of__parse_of_name
                   : forall h' (pf : h' < S (S h)) {str0 str valid name}
-                           (Hinit : sub_names_listT valid initial_names_data)
                            (p : parse_of String G str (Lookup G name)),
                       @of_parse_name_T str0 str valid name p h')
                  {struct h}
@@ -751,16 +747,12 @@ Section cfg.
       End production.
 
       Section productions.
-        (*Axiom minimal_parse_of_production__of__parse_of_production
-        : forall str h, of_parse_production_T str h.*)
-        Context {str0 str : String} {valid : names_listT}
-                (Hinit : sub_names_listT valid initial_names_data).
+        Context {str0 str : String} {valid : names_listT}.
 
         Fixpoint minimal_parse_of_productions__of__parse_of_productions
                  h
                  (minimal_parse_of_name__of__parse_of_name
                   : forall h' (pf : h' < S h) {str0 str valid name}
-                           (Hinit : sub_names_listT valid initial_names_data)
                            (p : parse_of String G str (Lookup G name)),
                       @of_parse_name_T str0 str valid name p h')
                  {struct h}
@@ -770,9 +762,10 @@ Section cfg.
           destruct h as [|h']; [ exfalso; omega | ].
           destruct p as [str' pat pats p' | str' pat pats p'].
           { clear minimal_parse_of_productions__of__parse_of_productions.
-            edestruct (minimal_parse_of_production__of__parse_of_production (h := h') minimal_parse_of_name__of__parse_of_name pf valid' Hinit' p') as [ [p'' p''H] | [name' H'] ];
+            edestruct (@minimal_parse_of_production__of__parse_of_production _ h' minimal_parse_of_name__of__parse_of_name _ pf valid' _ p') as [ [p'' p''H] | [name' H'] ];
             try solve [ exact (Lt.lt_S_n _ _ H_h)
-                      | exact H_forall ];
+                      | exact H_forall
+                      | exact Hinit' ];
             [|].
             { left.
               exists (MinParseHead pats p'').
@@ -794,6 +787,7 @@ Section cfg.
                              h' (transitivity pf (Lt.lt_n_Sn _))).
             edestruct (minimal_parse_of_productions__of__parse_of_productions h'  minimal_parse_of_name__of__parse_of_name _ pf valid' _ p') as [ [p'' p''H] | [name' H'] ];
             try solve [ exact (Lt.lt_S_n _ _ H_h)
+                      | exact Hinit'
                       | exact H_forall ];
             [|].
             { left.
@@ -817,24 +811,21 @@ Section cfg.
       Section name.
         Section step.
           Definition minimal_parse_of_name__of__parse_of_name_step
-                     {str}
                      h
                      (minimal_parse_of_name__of__parse_of_name
                       : forall h' (pf : h' < h) {str0 str valid name}
-                               (Hinit : sub_names_listT valid initial_names_data)
                                (p : parse_of String G str (Lookup G name)),
                           @of_parse_name_T str0 str valid name p h')
-                     {str0 valid name}
-                     (Hinit : sub_names_listT valid initial_names_data)
+                     {str0 str valid name}
                      (p : parse_of String G str (Lookup G name))
           : @of_parse_name_T str0 str valid name p h.
           Proof.
             destruct h as [|h]; [ clear; repeat intro; exfalso; omega | ].
-            intros pf Hstr H_forall.
+            intros pf Hstr Hinit' H_forall.
             let H := match goal with H : str ≤s str0 |- _ => constr:H end in
             destruct (strle_to_sumbool _ H) as [pf_lt|pf_eq].
             { (** [str] got smaller, so we reset the valid names list *)
-              destruct (@minimal_parse_of_productions__of__parse_of_productions str h minimal_parse_of_name__of__parse_of_name str (reflexivity _) initial_names_data (Lookup G name) p (Lt.lt_S_n _ _ pf) (snd H_forall)) as [p'|p'].
+              destruct (@minimal_parse_of_productions__of__parse_of_productions str h minimal_parse_of_name__of__parse_of_name str (reflexivity _) initial_names_data (Lookup G name) p (Lt.lt_S_n _ _ pf) (reflexivity _) (snd H_forall)) as [p'|p'].
               { left.
                 exists (MinParseNonTerminalStrLt _ valid _ pf_lt (projT1 p'));
                   simpl.
@@ -851,7 +842,7 @@ Section cfg.
                       | reflexivity ]. } }
             { (** [str] didn't get smaller, so we cache the fact that we've hit this name already *)
               destruct (Sumbool.sumbool_of_bool (is_valid_name valid name)) as [ Hvalid | Hinvalid ].
-              { destruct (@minimal_parse_of_productions__of__parse_of_productions str h minimal_parse_of_name__of__parse_of_name str (reflexivity _) (remove_name valid name) (Lookup G name) p (Lt.lt_S_n _ _ pf) (snd H_forall)) as [p'|p'].
+              { destruct (@minimal_parse_of_productions__of__parse_of_productions str h minimal_parse_of_name__of__parse_of_name str (reflexivity _) (remove_name valid name) (Lookup G name) p (Lt.lt_S_n _ _ pf) (transitivity (@sub_names_listT_remove _ _) Hinit') (snd H_forall)) as [p'|p'].
                 { left.
                   subst str.
                   eexists (MinParseNonTerminalStrEq Hvalid (projT1 p')).
@@ -864,9 +855,10 @@ Section cfg.
                 { destruct p' as [name' p'].
                   destruct (string_dec name name') as [|n].
                   { subst name; simpl in *.
-                    edestruct (minimal_parse_of_name__of__parse_of_name (S (size_of_parse p)) pf str0 valid name' Hinit (projT1 (snd p'))) as [p''|p''];
+                    edestruct (@minimal_parse_of_name__of__parse_of_name (S (size_of_parse p)) pf str0 _ valid name' (projT1 (snd p'))) as [p''|p''];
                     try solve [ apply Lt.lt_n_S, (fst (projT2 (snd p')))
                               | subst; reflexivity
+                              | assumption
                               | split; [ exact (proj2 (fst p'))
                                        | exact (snd (projT2 (snd p'))) ] ];
                     [|].
@@ -911,586 +903,18 @@ Section cfg.
 
         Section wf.
           Definition minimal_parse_of_name__of__parse_of_name
-                     {str}
           : forall h
-                   {str0 valid name}
-                   (Hinit : sub_names_listT valid initial_names_data)
+                   {str0 str valid name}
                    (p : parse_of String G str (Lookup G name)),
               @of_parse_name_T str0 str valid name p h
             := @Fix
                  _ lt lt_wf
-                 (fun h => forall {str0 valid name}
-                                  (Hinit : sub_names_listT valid initial_names_data)
+                 (fun h => forall {str0 str valid name}
                                   (p : parse_of String G str (Lookup G name)),
                              @of_parse_name_T str0 str valid name p h)
-                 (@minimal_parse_of_name__of__parse_of_name_step str).
+                 (@minimal_parse_of_name__of__parse_of_name_step).
         End wf.
-
-          Definition parse_name_step
-                     (str : String) (pf : str ≤s str0) (name : string)
-          : bool
-            := match lt_dec (Length str) (Length str0), Sumbool.sumbool_of_bool (is_valid_name valid_list name) with
-                 | left pf', _ =>
-                   (** [str] got smaller, so we reset the valid names list *)
-                   parse_productions
-                     (@parse_name
-                        (str, initial_names_data)
-                        (or_introl pf'))
-                     (or_intror eq_refl)
-                     (Lookup G name)
-                 | right pf', left H' =>
-                   (** [str] didn't get smaller, so we cache the fact that we've hit this name already *)
-                   (** It was valid, so we can remove it *)
-                   parse_productions
-                     (@parse_name
-                        (str0, remove_name valid_list name)
-                        (or_intror (conj eq_refl (remove_name_dec H'))))
-                     (or_intror eq_refl)
-                     (Lookup G name)
-                 | right _, right _
-                   => (** oops, we already saw this name in the past.  ABORT! *)
-                   false
-               end.
-        End step.
-
-        Section wf.
-          (** TODO: add comment explaining signature *)
-          Definition parse_name_or_abort
-          : forall (p : String * names_listT) (str : String),
-              str ≤s fst p
-              -> string
-              -> bool
-            := @Fix3
-                 (prod String names_listT) _ _ _
-                 _ (@well_founded_prod_relation
-                      String
-                      names_listT
-                      _
-                      _
-                      (well_founded_ltof _ Length)
-                      ntl_wf)
-                 _
-                 (fun sl => @parse_name_step (fst sl) (snd sl)).
-
-          Definition parse_name (str : String) (name : string)
-          : bool
-            := @parse_name_or_abort (str, initial_names_data) str
-                                    (or_intror eq_refl) name.
-        End wf.
-      End names.
-    End parts.
-  End bool.
-
-
-      Section item.
-        Context {str0 str : String} (valid : names_listT) {it : item CharType}.
-
-        Definition minimal_parse_of_item__of__parse_of_item
-                   h
-                   (minimal_parse_of_name__of__parse_of_name
-                    : forall name p, @of_parse_name_T str0 str valid name p h)
-                   (p : parse_of_item String G str it)
-        : @of_parse_item_T str0 str valid it p h.
-        Proof.
-          intros pf H_forall.
-          destruct p as [|name str' p'].
-          { left.
-            eexists (MinParseTerminal _ _ _).
-            split; simpl; solve [ constructor ]. }
-          { eapply minimal_parse_of_name__of__parse_of_name; try assumption. }
-        Defined.
-      End item.
-
-
-
-      Section production.
-        Let of_parse_production_T {str0 str valid pat} (p : parse_of_production String G str pat) h
-          := size_of_parse_production p < h
-             -> Forall_parse_of_production P p
-             -> ({ p' : minimal_parse_of_production str0 valid str pat
-                        & (size_of_parse_production (parse_of_production__of__minimal_parse_of_production p') <= size_of_parse_production p)
-                          * Forall_parse_of_production P (parse_of_production__of__minimal_parse_of_production p') })%type
-                + alt_option (size_of_parse_production p) valid str.
-
-        (*Let rec_T h
-          := forall h', h' < h -> of_parse_T h' -> forall str valid pat p, @of_parse_production_T str valid pat p h'.*)
-
-        Section helper.
-          Context (h : nat)
-                  (minimal_parse_of_production__of__parse_of_production_rec : rec_T h)
-                  (minimal_parse_of__of__parse_of : of_parse_T h).
-
-          Let minimal_parse_of_production__of__parse_of_production h' H
-          : forall {str} valid {pat} (p : parse_of_production String G str pat),
-              of_parse_production_T p h'
-            := @minimal_parse_of_production__of__parse_of_production_rec
-                 h' H (of_parse_T_resp H (@minimal_parse_of__of__parse_of)).
-
-          Let minimal_parse_of_item__of__parse_of_item {str} valid {it}
-            := @minimal_parse_of_item__of__parse_of_item' str valid it h minimal_parse_of__of__parse_of.
-
-          Context {str : String} (valid : names_listT) {pat : production CharType}.
-
-          Definition minimal_parse_of_production__of__parse_of_production'_helper
-                     (p : parse_of_production String G str pat)
-          : @of_parse_production_T str valid pat p h.
-          Proof.
-            refine (
-                match h as h, p as p in (parse_of_production _ _ str pat)
-                      return ((forall h' (H : h' < h) str valid pat (p : parse_of_production String G str pat),
-                                 of_parse_production_T p h')
-                              -> (forall str valid it p', @of_parse_item_T str valid it p' h) -> of_parse_production_T p h)
-                with
-                  | 0, _ => fun _ _ H' _ => match Lt.lt_n_0 _ H' : False with end
-                  | S h', ParseProductionNil
-                    => fun _ _ p_small forall_parse
-                       => inl (existT
-                                 _ (MinParseProductionNil _)
-                                 (reflexivity _, forall_parse))
-                  | S h', ParseProductionCons str0 pat' str1 pats' p0' p1'
-                    => fun minimal_parse_of_production__of__parse_of_production
-                           minimal_parse_of_item__of__parse_of_item
-                           p_small forall_parse
-                       => let mp0 := @minimal_parse_of_item__of__parse_of_item _ valid _ p0' (NPeano.Nat.lt_succ_l _ _ (proj1 (proj1 (NPeano.Nat.max_lub_lt_iff _ _ _) p_small))) (fst forall_parse) in
-                          let mp0' := alt_all_elim (@minimal_parse_of_item__of__parse_of_item _ initial_names_data _ p0' (NPeano.Nat.lt_succ_l _ _ (proj1 (proj1 (NPeano.Nat.max_lub_lt_iff _ _ _) p_small))) (fst forall_parse)) in
-                          let mp1 := (@minimal_parse_of_production__of__parse_of_production _ p_small _ valid _ p1' (Max.le_max_r _ _) (snd forall_parse)) in
-                          let mp1' := alt_all_elim (@minimal_parse_of_production__of__parse_of_production _ p_small _ initial_names_data _ p1' (Max.le_max_r _ _) (snd forall_parse)) in
-                          match stringlike_dec str0 (Empty _), stringlike_dec str1 (Empty _) with
-                            | right pf0, right pf1
-                              => inl (existT
-                                        _ (MinParseProductionConsDec valid pf0 pf1 (projT1 mp0') (projT1 mp1'))
-                                        (NPeano.Nat.max_le_compat _ _ _ _ (Le.le_n_S _ _ (fst (projT2 mp0'))) (Le.le_n_S _ _ (fst (projT2 mp1'))),
-                                         (snd (projT2 mp0'), snd (projT2 mp1'))))
-                            | left pf0, left pf1
-                              => let eq_pf0 := (_ : str0 = str0 ++ str1) in
-                                 let eq_pf1 := (_ : str1 = str0 ++ str1) in
-                                 match mp0, mp1 with
-                                   | inl mp0'', inl mp1''
-                                     => inl (existT
-                                               _ (MinParseProductionConsEmpty01 pf0 pf1 (projT1 mp0'') (projT1 mp1''))
-                                               (NPeano.Nat.max_le_compat _ _ _ _ (Le.le_n_S _ _ (fst (projT2 mp0''))) (Le.le_n_S _ _ (fst (projT2 mp1''))),
-                                                (snd (projT2 mp0''), snd (projT2 mp1''))))
-                                   | inr other, _
-                                     => inr (expand_alt_option
-                                               (Max.le_max_l _ _)
-                                               (reflexivity _)
-                                               eq_pf0
-                                               other)
-                                   | _, inr other
-                                     => inr (expand_alt_option
-                                               (Max.le_max_r _ _)
-                                               (reflexivity _)
-                                               eq_pf1
-                                               other)
-                                 end
-                            | left pf0, right pf1
-                              => let eq_pf := (_ : str1 = str0 ++ str1) in
-                                 match mp1 with
-                                   | inl mp1''
-                                     => inl (existT
-                                               _ (MinParseProductionConsEmpty0 pf0 pf1 (projT1 mp0') (projT1 mp1''))
-                                               (NPeano.Nat.max_le_compat _ _ _ _ (Le.le_n_S _ _ (fst (projT2 mp0'))) (Le.le_n_S _ _ (fst (projT2 mp1''))),
-                                                (snd (projT2 mp0'), snd (projT2 mp1''))))
-                                   | inr other
-                                     => inr (expand_alt_option
-                                               (Max.le_max_r _ _)
-                                               (reflexivity _)
-                                               eq_pf
-                                               other)
-                                 end
-                            | right pf0, left pf1
-                              => let eq_pf := (_ : str0 = str0 ++ str1) in
-                                 match mp0 with
-                                   | inl mp0''
-                                     => inl (existT
-                                               _ (MinParseProductionConsEmpty1 pf0 pf1 (projT1 mp0'') (projT1 mp1'))
-                                               (NPeano.Nat.max_le_compat _ _ _ _ (Le.le_n_S _ _ (fst (projT2 mp0''))) (Le.le_n_S _ _ (fst (projT2 mp1'))),
-                                                (snd (projT2 mp0''), snd (projT2 mp1'))))
-                                   | inr other
-                                     => inr (expand_alt_option
-                                               (Max.le_max_l _ _)
-                                               (reflexivity _)
-                                               eq_pf
-                                               other)
-                                 end
-                          end
-                end
-                  (@minimal_parse_of_production__of__parse_of_production)
-                  (@minimal_parse_of_item__of__parse_of_item));
-            simpl in *;
-            try solve [ subst; rewrite ?LeftId, ?RightId; trivial ].
-          Defined.
-        End helper.
-
-
-        (*Let rec_T str0 str pf it h
-          := forall h', h' < h -> of_parse_T h' -> forall p, @of_parse_item_T str0 str pf valid it p h'.
-
-        Section helper.
-          Context (h : nat)
-                  (minimal_parse_of_item__of__parse_of_item_rec : rec_T pf it h)
-                  (minimal_parse_of__of__parse_of : of_parse_T h).
-
-          Definition minimal_parse_of_item__of__parse_of_item'_helper
-                     (p : parse_of_item String G str it)
-          : @of_parse_item_T str0 str pf valid it p h.
-            refine
-              (match h as h, p as p in (parse_of_item _ _ str it)
-                     return (forall pf : str ≤s str0,
-                               @rec_T str0 str pf it h
-                               -> @of_parse_T h
-                               -> @of_parse_item_T str0 str pf valid it p h)
-               with
-                 | _, ParseTerminal x
-                   => fun pf _ _ H' _ => inl (existT _ (@MinParseTerminal str0 valid x pf) (le_n _, tt))
-                 | 0, ParseNonTerminal _ _ _
-                   => fun _ _ _ H' _ => match Lt.lt_n_0 _ H' : False with end
-                 | S h', ParseNonTerminal name str' p'
-                   => fun pf
-                          minimal_parse_of_item__of__parse_of_item_rec
-                          minimal_parse_of__of__parse_of
-                          p_small forall_parse
-                      => _
-               end
-                 pf
-                 (@minimal_parse_of_item__of__parse_of_item_rec)
-                 (@minimal_parse_of__of__parse_of)).
-            exists ).
-inl (existT _ (MinParseTerminal _ x) )
-                 | S h',
-                   => fun minimal_parse_of_item__of__parse_of_item_rec
-                          minimal_parse_of__of__parse_of
-                          p_small forall_parse
-                      => match @minimal_parse_of__of__parse_of
-                                 _ (remove_name valid name) _
-                                 p'
-                                 (NPeano.Nat.lt_succ_l _ _ p_small)
-                                 (snd forall_parse)
-                         with
-                           | inl (existT mp (H0, H0_forall))
-                             => match Sumbool.sumbool_of_bool (is_valid_name valid name) with
-                                  | left H'
-                                    => inl (existT _ (MinParseNonTerminal H' mp) (Le.le_n_S _ _ H0, (fst forall_parse, H0_forall)))
-                                  | right H'
-                                    => inr (existT
-                                              _ name
-                                              (conj H' (fst forall_parse),
-                                               existT
-                                                 _ (parse_of__of__minimal_parse_of mp)
-                                                 (Lt.le_lt_n_Sm _ _ H0, H0_forall)))
-                                end
-                           | inr (existT name' other)
-                             => match string_dec name name' with
-                                  | right pf
-                                    => inr (existT
-                                              _ name'
-                                              (conj
-                                                 (eq_trans (eq_sym (remove_name_5 valid pf)) (proj1 (fst other)))
-                                                 (proj2 (fst other)),
-                                               (existT
-                                                  _ (projT1 (snd other))
-                                                  (Lt.lt_S _ _ (fst (projT2 (snd other))), snd (projT2 (snd other))))))
-                                  | left pf
-                                    => match Sumbool.sumbool_of_bool (is_valid_name valid name) with
-                                         | left H'
-                                           => let other' :=
-                                                  (match eq_sym pf in (_ = y)
-                                                         return (is_valid_name (remove_name valid name) y =
-                                                                 false /\ P y) *
-                                                                { p0 : parse_of String G _ (Lookup G y)
-                                                                       & ((size_of_parse p0 < size_of_parse _) * Forall_parse_of P p0)%type }
-                                                   with
-                                                     | eq_refl => other
-                                                   end) in
-                                              let p'' := (@minimal_parse_of_item__of__parse_of_item_rec
-                                                            _ p_small
-                                                            (of_parse_T_resp p_small minimal_parse_of__of__parse_of)
-                                                            (ParseNonTerminal name (projT1 (snd other')))
-                                                            (Lt.lt_n_S _ _ (fst (projT2 (snd other'))))
-                                                            (proj2 (fst other'), snd (projT2 (snd other')))) in
-
-                                              match p'' with
-                                                | inl (existT p''' (H'', H''_forall))
-                                                  => inl (existT
-                                                            _ p'''
-                                                            (Le.le_trans _ _ _ H'' (Lt.lt_le_weak _ _ (Lt.lt_n_S _ _ (fst (projT2 (snd other'))))), H''_forall))
-                                                | inr p'''
-                                                  => inr (expand_alt_option
-                                                            (Lt.lt_n_S _ _ (fst (projT2 (snd other'))))
-                                                            (reflexivity _)
-                                                            (reflexivity _)
-                                                            p''')
-                                              end
-                                         | right H'
-                                           => inr (existT
-                                                     _ name'
-                                                     (conj
-                                                        (match pf in (_ = y)
-                                                               return is_valid_name valid y = false
-                                                         with
-                                                           | eq_refl => H'
-                                                         end)
-                                                        (proj2 (fst other)),
-                                                      (existT
-                                                         _ (projT1 (snd other))
-                                                         (Lt.lt_S _ _ (fst (projT2 (snd other))), snd (projT2 (snd other))))))
-                                       end
-                                end
-                         end
-               end
-                 (@minimal_parse_of_item__of__parse_of_item_rec)
-                 (@minimal_parse_of__of__parse_of)).
-        End helper.
-
-        Definition minimal_parse_of_item__of__parse_of_item'
-        : forall (h : nat)
-                 (minimal_parse_of__of__parse_of : of_parse_T h)
-                 (p : parse_of_item String G str it),
-            of_parse_item_T p h
-          := Fix Wf_nat.lt_wf _ minimal_parse_of_item__of__parse_of_item'_helper.
-      End item.
-
-      Section production.
-        Let of_parse_production_T {str valid pat} (p : parse_of_production String G str pat) h
-          := size_of_parse_production p < h
-             -> Forall_parse_of_production P p
-             -> ({ p' : minimal_parse_of_production valid str pat
-                        & (size_of_parse_production (parse_of_production__of__minimal_parse_of_production p') <= size_of_parse_production p)
-                          * Forall_parse_of_production P (parse_of_production__of__minimal_parse_of_production p') })%type
-                + alt_option (size_of_parse_production p) valid str.
-
-        Let rec_T h
-          := forall h', h' < h -> of_parse_T h' -> forall str valid pat p, @of_parse_production_T str valid pat p h'.
-
-        Section helper.
-          Context (h : nat)
-                  (minimal_parse_of_production__of__parse_of_production_rec : rec_T h)
-                  (minimal_parse_of__of__parse_of : of_parse_T h).
-
-          Let minimal_parse_of_production__of__parse_of_production h' H
-          : forall {str} valid {pat} (p : parse_of_production String G str pat),
-              of_parse_production_T p h'
-            := @minimal_parse_of_production__of__parse_of_production_rec
-                 h' H (of_parse_T_resp H (@minimal_parse_of__of__parse_of)).
-
-          Let minimal_parse_of_item__of__parse_of_item {str} valid {it}
-            := @minimal_parse_of_item__of__parse_of_item' str valid it h minimal_parse_of__of__parse_of.
-
-          Context {str : String} (valid : names_listT) {pat : production CharType}.
-
-          Definition minimal_parse_of_production__of__parse_of_production'_helper
-                     (p : parse_of_production String G str pat)
-          : @of_parse_production_T str valid pat p h.
-          Proof.
-            refine (
-                match h as h, p as p in (parse_of_production _ _ str pat)
-                      return ((forall h' (H : h' < h) str valid pat (p : parse_of_production String G str pat),
-                                 of_parse_production_T p h')
-                              -> (forall str valid it p', @of_parse_item_T str valid it p' h) -> of_parse_production_T p h)
-                with
-                  | 0, _ => fun _ _ H' _ => match Lt.lt_n_0 _ H' : False with end
-                  | S h', ParseProductionNil
-                    => fun _ _ p_small forall_parse
-                       => inl (existT
-                                 _ (MinParseProductionNil _)
-                                 (reflexivity _, forall_parse))
-                  | S h', ParseProductionCons str0 pat' str1 pats' p0' p1'
-                    => fun minimal_parse_of_production__of__parse_of_production
-                           minimal_parse_of_item__of__parse_of_item
-                           p_small forall_parse
-                       => let mp0 := @minimal_parse_of_item__of__parse_of_item _ valid _ p0' (NPeano.Nat.lt_succ_l _ _ (proj1 (proj1 (NPeano.Nat.max_lub_lt_iff _ _ _) p_small))) (fst forall_parse) in
-                          let mp0' := alt_all_elim (@minimal_parse_of_item__of__parse_of_item _ initial_names_data _ p0' (NPeano.Nat.lt_succ_l _ _ (proj1 (proj1 (NPeano.Nat.max_lub_lt_iff _ _ _) p_small))) (fst forall_parse)) in
-                          let mp1 := (@minimal_parse_of_production__of__parse_of_production _ p_small _ valid _ p1' (Max.le_max_r _ _) (snd forall_parse)) in
-                          let mp1' := alt_all_elim (@minimal_parse_of_production__of__parse_of_production _ p_small _ initial_names_data _ p1' (Max.le_max_r _ _) (snd forall_parse)) in
-                          match stringlike_dec str0 (Empty _), stringlike_dec str1 (Empty _) with
-                            | right pf0, right pf1
-                              => inl (existT
-                                        _ (MinParseProductionConsDec valid pf0 pf1 (projT1 mp0') (projT1 mp1'))
-                                        (NPeano.Nat.max_le_compat _ _ _ _ (Le.le_n_S _ _ (fst (projT2 mp0'))) (Le.le_n_S _ _ (fst (projT2 mp1'))),
-                                         (snd (projT2 mp0'), snd (projT2 mp1'))))
-                            | left pf0, left pf1
-                              => let eq_pf0 := (_ : str0 = str0 ++ str1) in
-                                 let eq_pf1 := (_ : str1 = str0 ++ str1) in
-                                 match mp0, mp1 with
-                                   | inl mp0'', inl mp1''
-                                     => inl (existT
-                                               _ (MinParseProductionConsEmpty01 pf0 pf1 (projT1 mp0'') (projT1 mp1''))
-                                               (NPeano.Nat.max_le_compat _ _ _ _ (Le.le_n_S _ _ (fst (projT2 mp0''))) (Le.le_n_S _ _ (fst (projT2 mp1''))),
-                                                (snd (projT2 mp0''), snd (projT2 mp1''))))
-                                   | inr other, _
-                                     => inr (expand_alt_option
-                                               (Max.le_max_l _ _)
-                                               (reflexivity _)
-                                               eq_pf0
-                                               other)
-                                   | _, inr other
-                                     => inr (expand_alt_option
-                                               (Max.le_max_r _ _)
-                                               (reflexivity _)
-                                               eq_pf1
-                                               other)
-                                 end
-                            | left pf0, right pf1
-                              => let eq_pf := (_ : str1 = str0 ++ str1) in
-                                 match mp1 with
-                                   | inl mp1''
-                                     => inl (existT
-                                               _ (MinParseProductionConsEmpty0 pf0 pf1 (projT1 mp0') (projT1 mp1''))
-                                               (NPeano.Nat.max_le_compat _ _ _ _ (Le.le_n_S _ _ (fst (projT2 mp0'))) (Le.le_n_S _ _ (fst (projT2 mp1''))),
-                                                (snd (projT2 mp0'), snd (projT2 mp1''))))
-                                   | inr other
-                                     => inr (expand_alt_option
-                                               (Max.le_max_r _ _)
-                                               (reflexivity _)
-                                               eq_pf
-                                               other)
-                                 end
-                            | right pf0, left pf1
-                              => let eq_pf := (_ : str0 = str0 ++ str1) in
-                                 match mp0 with
-                                   | inl mp0''
-                                     => inl (existT
-                                               _ (MinParseProductionConsEmpty1 pf0 pf1 (projT1 mp0'') (projT1 mp1'))
-                                               (NPeano.Nat.max_le_compat _ _ _ _ (Le.le_n_S _ _ (fst (projT2 mp0''))) (Le.le_n_S _ _ (fst (projT2 mp1'))),
-                                                (snd (projT2 mp0''), snd (projT2 mp1'))))
-                                   | inr other
-                                     => inr (expand_alt_option
-                                               (Max.le_max_l _ _)
-                                               (reflexivity _)
-                                               eq_pf
-                                               other)
-                                 end
-                          end
-                end
-                  (@minimal_parse_of_production__of__parse_of_production)
-                  (@minimal_parse_of_item__of__parse_of_item));
-            simpl in *;
-            try solve [ subst; rewrite ?LeftId, ?RightId; trivial ].
-          Defined.
-        End helper.
-
-        Definition minimal_parse_of_production__of__parse_of_production'
-        : forall (h : nat)
-                 (minimal_parse_of__of__parse_of : of_parse_T h)
-                 {str} valid {pat}
-                 (p : parse_of_production String G str pat),
-            @of_parse_production_T str valid pat p h
-          := Fix Wf_nat.lt_wf _ minimal_parse_of_production__of__parse_of_production'_helper.
-      End production.
-
-      Section parse_of.
-        Let rec_T h
-          := forall h', h' < h -> of_parse_T h'.
-
-        Section helper.
-          Context (h : nat)
-                  (minimal_parse_of__of__parse_of_rec : rec_T h).
-
-          Let minimal_parse_of__of__parse_of h' H
-          : of_parse_T h'
-            := @minimal_parse_of__of__parse_of_rec h' H.
-
-          Context {str : String} (valid : names_listT) {pats : productions CharType}.
-
-          Definition minimal_parse_of__of__parse_of'_helper
-                     (p : parse_of String G str pats)
-          : @of_parse_T' h str valid pats p
-            := match h as h, p as p in (parse_of _ _ str pats)
-                     return ((forall h' (H : h' < h), of_parse_T h')
-                             -> @of_parse_T' h str valid pats p)
-               with
-                 | 0, _ => fun _ H' => match Lt.lt_n_0 _ H' : False with end
-                 | S h', ParseHead _ pat' pats' p'
-                   => fun minimal_parse_of__of__parse_of
-                          p_small
-                          forall_parse
-                      => let minimal_parse_of_production__of__parse_of_production
-                               {str} valid {pat}
-                             := @minimal_parse_of_production__of__parse_of_production' h' (@minimal_parse_of__of__parse_of _ (Lt.lt_n_Sn _)) str valid pat in
-                         match minimal_parse_of_production__of__parse_of_production valid p' (Lt.lt_S_n _ _ p_small) forall_parse with
-                           | inl mp
-                             => inl (existT
-                                       _ (MinParseHead pats' (projT1 mp))
-                                       (Le.le_n_S _ _ (fst (projT2 mp)),
-                                        snd (projT2 mp)))
-                           | inr other
-                             => inr (expand_alt_option
-                                       (Lt.lt_n_Sn _)
-                                       (reflexivity _)
-                                       (reflexivity _)
-                                       other)
-                         end
-                 | S h', ParseTail _ pat' pats' p'
-                   => fun minimal_parse_of__of__parse_of
-                          p_small
-                          forall_parse
-                      => match minimal_parse_of__of__parse_of _ (Lt.lt_n_Sn _) _ valid _ p' (Lt.lt_S_n _ _ p_small) forall_parse with
-                           | inl mp
-                             => inl (existT
-                                       _ (MinParseTail pat' (projT1 mp))
-                                       (Le.le_n_S _ _ (fst (projT2 mp)),
-                                        snd (projT2 mp)))
-                           | inr other
-                             => inr (expand_alt_option
-                                       (Lt.lt_n_Sn _)
-                                       (reflexivity _)
-                                       (reflexivity _)
-                                       other)
-                         end
-               end
-                 (@minimal_parse_of__of__parse_of).
-        End helper.
-
-        Definition minimal_parse_of__of__parse_of'
-        : forall (h : nat)
-                 {str} valid {pats}
-                 (p : parse_of String G str pats),
-            @of_parse_T' h str valid pats p
-          := Fix Wf_nat.lt_wf _ minimal_parse_of__of__parse_of'_helper.
-      End parse_of.
+      End name.
     End wf_parts.
-
-    Definition minimal_parse_of__of__parse_of
-               {str : String} {pats : productions CharType}
-               (p : parse_of String G str pats)
-               (H : Forall_parse_of P p)
-    : minimal_parse_of initial_names_data str pats
-      := match @minimal_parse_of__of__parse_of'
-                 _ str initial_names_data pats p
-                 (Lt.lt_n_Sn _)
-                 H with
-           | inl p' => projT1 p'
-           | inr other => let H' := fst (projT2 other) in
-                          match Bool.eq_true_false_abs _ (proj2 H') (proj1 H') : False with end
-         end.
-
-    Definition minimal_parse_of_production__of__parse_of_production
-               {str : String} {pat : production CharType}
-               (p : parse_of_production String G str pat)
-               (H : Forall_parse_of_production P p)
-    : minimal_parse_of_production initial_names_data str pat
-      := match @minimal_parse_of_production__of__parse_of_production'
-                 _ (@minimal_parse_of__of__parse_of' _) str initial_names_data pat p
-                 (Lt.lt_n_Sn _)
-                 H with
-           | inl p' => projT1 p'
-           | inr other => let H' := fst (projT2 other) in
-                          match Bool.eq_true_false_abs _ (proj2 H') (proj1 H') : False with end
-         end.
-
-    Definition minimal_parse_of_item__of__parse_of_item
-               {str : String} {it : item CharType}
-               (p : parse_of_item String G str it)
-               (H : Forall_parse_of_item P p)
-    : minimal_parse_of_item initial_names_data str it
-      := match @minimal_parse_of_item__of__parse_of_item'
-                 str initial_names_data it
-                 _ (@minimal_parse_of__of__parse_of' _) p
-                 (Lt.lt_n_Sn _)
-                 H with
-           | inl p' => projT1 p'
-           | inr other => let H' := fst (projT2 other) in
-                          match Bool.eq_true_false_abs _ (proj2 H') (proj1 H') : False with end
-         end.
   End minimize.
 End cfg.
